src/cddl/pulse/CDDL.Pulse.Serialize.Gen.MapGroup.ZeroOrMore.Aux2.Lemma13.fsti
@@ -28,6 +28,11 @@ val invariant_insert_dup
   (v0 v: Map.t tkey (list tvalue))
   (min: nat)
   (max: option nat)
+  (vout_old: Ghost.erased (Seq.seq U8.t))
+  (gk: Ghost.erased tkey)
+  (gv: Ghost.erased tvalue)
+  (min_old: Ghost.erased nat)
+  (max_old: Ghost.erased (option nat))
 : Lemma
   (requires
     em == false /\
@@ -37,13 +42,13 @@ val invariant_insert_dup
     map_of_list_maps_to_nonempty v /\
     impl_serialize_map_zero_or_more_iterator_gen_invariant_min p sp1 sp2 except min v0 v /\
     impl_serialize_map_zero_or_more_iterator_gen_invariant_max p sp1 sp2 except max v0 v /\
-    (exists (vout_old: Seq.seq U8.t) (gk: tkey) (gv: tvalue) (key_eq: EqTest.eq_test tkey) (min_old: nat) (max_old: option nat) .
-      impl_serialize_map_zero_or_more_iterator_gen_invariant p sp1 sp2 except em out vout_old size count m v0 (map_of_list_cons key_eq gk gv v) min_old max_old true /\
-      min == impl_serialize_map_zero_or_more_iterator_gen_update_min minl sp1 sp2 except min_old gk gv /\
-      max == impl_serialize_map_zero_or_more_iterator_gen_update_max maxl sp1 sp2 except max_old gk gv /\
-      sp1.serializable gk /\ sp2.serializable gv /\
-      except (sp1.serializer gk, sp2.serializer gv) == false /\
-      cbor_map_defined (sp1.serializer gk) m)
+    (exists (keq: EqTest.eq_test tkey) .
+      impl_serialize_map_zero_or_more_iterator_gen_invariant p sp1 sp2 except em out (Ghost.reveal vout_old) size count m v0 (map_of_list_cons keq (Ghost.reveal gk) (Ghost.reveal gv) v) (Ghost.reveal min_old) (Ghost.reveal max_old) true /\
+      min == impl_serialize_map_zero_or_more_iterator_gen_update_min minl sp1 sp2 except (Ghost.reveal min_old) (Ghost.reveal gk) (Ghost.reveal gv) /\
+      max == impl_serialize_map_zero_or_more_iterator_gen_update_max maxl sp1 sp2 except (Ghost.reveal max_old) (Ghost.reveal gk) (Ghost.reveal gv) /\
+      sp1.serializable (Ghost.reveal gk) /\ sp2.serializable (Ghost.reveal gv) /\
+      except (sp1.serializer (Ghost.reveal gk), sp2.serializer (Ghost.reveal gv)) == false /\
+      cbor_map_defined (sp1.serializer (Ghost.reveal gk)) m)
   )
   (ensures
     impl_serialize_map_zero_or_more_iterator_gen_invariant p sp1 sp2 except em out vout size count m v0 v min max false
